

Problem 1.

Show that  $\partial\phi/\partial x^\mu$  is a covariant four-vector ( $\phi$  is a scalar function of  $x$ ,  $y$ ,  $z$ , and  $t$ ).

Hint: First determine (from Equation 3.8) how covariant four-vectors transform; then use  $\partial\phi / \partial x^{\mu'} = (\partial\phi / \partial x^\nu)(\partial x^\nu / \partial x^{\mu'})$  transforms.

Solution

The four-vectors in  $x$ ,  $y$ ,  $z$ ,  $t$  :

$$x^0 = ct, x^1 = x, x^2 = y, x^3 = z. \text{ Equation (3.7)}$$

Equation (3.8)

$$\begin{aligned} x^{0'} &= \gamma(x^0 - \beta x^1) \\ x^{1'} &= \gamma(x^1 - \beta x^0) \\ x^{2'} &= x^2 \\ x^{3'} &= x^3 \\ x^{\mu'} &= \sum_{\nu=0}^3 \Lambda_{\nu}^{\mu'} x^{\nu} \quad (\nu = 0, 1, 2, 3) = \Lambda_{\nu}^{\mu'} x^{\nu} \end{aligned}$$

This is a contravariant tensor.

A contravariant tensor: axes changes  $\rightarrow$  the components **inversely** change. And the vector does not change.

This is why it is called contravariant tensor.

A covariant : axes changes  $\rightarrow$  the components also changes in the same way : vector  $\rightarrow$  scalar.

A covariant vectors' components change the same as coordinates' change.

From Equation 3.8,

$$x^{0'} = \gamma(x^0 - \beta x^1) \rightarrow x'_0 = \gamma(x^0 + \beta x^1)$$

(The details are in Equation 3.1 and 3.3 , 3.3 is the inverse transform of 3.1. using the same inverse transform here.)

$$x^{1'} = \gamma(x^1 - \beta x^0) \rightarrow x'_1 = \gamma(x^1 + \beta x^0)$$

$$x'_2 = x^2$$

$$x'_3 = x^3$$

These are the covariant transform.

Q. What is the scalar function  $\phi$ ?

The quantity  $I$  (in Equation 3.13) and  $r^2 = x^2 + y^2 + z^2$  can be scalar function.  
(not sure)

So, using,  $I = (x^{0'})^2 - (x^{1'})^2 - (x^{2'})^2 - (x^{3'})^2$ ,

Since  $I = x_\mu x^\mu$ ,

$\partial\phi / \partial x^{\mu'} = x_\mu$ , covariant tensor.

[https://en.wikipedia.org/wiki/covariance\\_and\\_contravariance\\_of\\_vectors](https://en.wikipedia.org/wiki/covariance_and_contravariance_of_vectors)

Problem 2

7.2 Show that Equation 7.17 satisfies Equation 7.15

Solution

Equation 7.15 :  $\{\gamma^\mu, \gamma^\nu\} = 2g^{\mu\nu}$

Equation 7.17 :  $\gamma^0 = \begin{pmatrix} 1 & 0 \\ 0 & -1 \end{pmatrix}, \gamma^i = \begin{pmatrix} 0 & \sigma^i \\ -\sigma^i & 0 \end{pmatrix}$

Anticommutator  $\{A, B\} = AB + BA$

So,

$$\{\gamma^0, \gamma^i\} = \gamma^0 \gamma^i + \gamma^i \gamma^0 =$$

$$\begin{pmatrix} 1 & 0 \\ 0 & -1 \end{pmatrix} \begin{pmatrix} 0 & \sigma^i \\ -\sigma^i & 0 \end{pmatrix} + \begin{pmatrix} 0 & \sigma^i \\ -\sigma^i & 0 \end{pmatrix} \begin{pmatrix} 1 & 0 \\ 0 & -1 \end{pmatrix}$$

$$= \begin{pmatrix} 0 & \sigma^i \\ -\sigma^i & 0 \end{pmatrix} + \begin{pmatrix} 0 & -\sigma^i \\ -\sigma^i & 0 \end{pmatrix} = \begin{pmatrix} 0 & 0 \\ -2\sigma^i & 0 \end{pmatrix}$$

So, is this  $2g^{0i}$  ?

$$\text{Equation (3.14) } g = \begin{pmatrix} 1 & 0 & 0 & 0 \\ 0 & -1 & 0 & 0 \\ 0 & 0 & -1 & 0 \\ 0 & 0 & 0 & -1 \end{pmatrix}$$

This is the minkowski metric,  $g_{\mu\nu}$ .

$g^{\mu\nu}$  is simply  $g^{-1}$ , and  $g = g^{-1}$  (from wiki-minkowski metric)